src/voteprivacy/lemma_25.v
@@ -1,202 +1,20 @@
 (************************************************************************)
-(* Copyright (c) 2017-2018, Ajay Kumar Eeralla <ae266@mail.missouri.edu>*) 
-(************************************************************************)     
+(* Copyright (c) 2017-2018, Ajay Kumar Eeralla <ae266@mail.missouri.edu>*)
+(************************************************************************)
 Require Export auxDefs.
 Import ListNotations.
-(* Module aux. *)
-(*   Export destructTerm. *)
-(*   Fixpoint submsg_bol pk r (t': message)(s: message) (b: Bool): Bool := *)
-(*     match b with *)
-(*     | eqb  b1 b2 =>  (eqb (submsg_bol pk r t' s b1) (submsg_bol pk r t' s b2)) *)
-(*     | eqm t1 t2 => (eqm (submsg_msg pk r t' s t1) (submsg_msg pk r t' s t2)) *)
-(*     | ifb_then_else_ t1 t2 t3 => (IF (submsg_bol pk r t' s t1) then (submsg_bol pk r t' s t2) else (submsg_bol pk r t' s t3)) *)
-(*     | ver t1 t2 t3 => ver (submsg_msg pk r t' s t1) (submsg_msg pk r t' s t2) (submsg_msg pk r t' s t3) *)
-(*     | bver t1 t2 t3 => bver (submsg_msg pk r t' s t1) (submsg_msg pk r t' s t2) (submsg_msg pk r t' s t3) *)
-(*     | acc t1 t2 t3 t4 => acc (submsg_msg pk r t' s t1) (submsg_msg pk r t' s t2) (submsg_msg pk r t' s t3) (submsg_msg pk r t' s t4) *)
-(*     | _ => b *)
-(*     end *)
-(*   with submsg_msg pk r (t': message)(s: message) (t: message): message := *)
-(*          match t with *)
-(*          | enc t1 t2 t3 => match t2, t3 with *)
-(*                            | pi1 (ke (nonce n1)), re (nonce n2) => if ((n1 =? pk)%nat && (n2 =? r)%nat)&& message_beq t1 t' *)
-(*                                                                    then enc s t2 t3 else t *)
-(*                            | _, _ => t *)
-(*                            end *)
-(*          | _ => t *)
-
-(*          end. *)
-
-(*   Fixpoint submsg_os pk r (t': message) (s: message) (os: oursum): oursum := *)
-(*     match os with *)
-(*     | msg t => msg (submsg_msg pk r t' s t) *)
-(*     | bol b => bol (submsg_bol pk r t' s b) *)
-(*     end. *)
-
-(*   Fixpoint submsgMylist pk r (t': message) (s: message) {n} (ml: mylist n): mylist n := *)
-(*     match ml with *)
-(*     | [] => [] *)
-(*     | h:t => (submsg_os pk r t' s h): submsgMylist pk r t' s t *)
-(*     end. *)
-
-(*   (* Replace nonce directly as the above definition seems slow  *) *)
-(*   Fixpoint repNonceBol n n' b: Bool := *)
-(*   match b with *)
-(*     | eqb  b1 b2 =>  (eqb (repNonceBol n n' b1) (repNonceBol n n' b2)) *)
-(*     | eqm t1 t2 => (eqm (repNonceMsg n n' t1) (repNonceMsg n n' t2)) *)
-(*     | ifb_then_else_ t1 t2 t3 => (IF (repNonceBol n n' t1) then (repNonceBol n n' t2) else (repNonceBol n n' t3)) *)
-(*     | ver t1 t2 t3 => ver  (repNonceMsg n n' t1) (repNonceMsg n n' t2) (repNonceMsg n n' t3) *)
-(*     | bver t1 t2 t3 => bver (repNonceMsg n n' t1) (repNonceMsg n n' t2) (repNonceMsg n n' t3) *)
-(*     | acc t1 t2 t3 t4 => acc (repNonceMsg n n' t1) (repNonceMsg n n' t2) (repNonceMsg n n' t3) (repNonceMsg n n' t4) *)
-(*     | _ => b *)
-(*   end *)
-(* with repNonceMsg n n' t: message := *)
-(*        match t with *)
-(*          | nonce k => if (k =? n)%nat then (nonce n') else t *)
-(*          | ifm_then_else_ b1 t1 t2 =>    (If (repNonceBol n n' b1) then (repNonceMsg n n' t1) else (repNonceMsg n n' t2)) *)
-(*          | pair t1 t2 => pair (repNonceMsg n n' t1) (repNonceMsg n n' t2) *)
-(*          | pi1 t1 =>  pi1 (repNonceMsg n n' t1) *)
-(*          | pi2 t1 =>  pi2 (repNonceMsg n n' t1) *)
-(*          | L t1 =>  L (repNonceMsg n n' t1) *)
-(*          | to t1 => to  (repNonceMsg n n' t1) *)
-(*          | f l =>  (f (@map message message  (repNonceMsg n n') l)) *)
-(*          (** foo function symbol *) *)
-(*          (** FOO syntax *) *)
-(*          (** Vote values *) *)
-(*          | V0 t1 => V0 (repNonceMsg n n' t1) *)
-(*          | V1 t1 => V1 (repNonceMsg n n' t1) *)
-(*          (** Public Key *) *)
-(*          | pubkey t1 => pubkey (repNonceMsg n n' t1) *)
-(*          (** Commitments *) *)
-(*          | kc t1 => kc (repNonceMsg n n' t1) *)
-(*          | comm t1 t2 => comm (repNonceMsg n n' t1) (repNonceMsg n n' t2) *)
-(*          | open t1 t2 t3 => open (repNonceMsg n n' t1) (repNonceMsg n n' t2) (repNonceMsg n n' t3) *)
-(*          (** Shuffling *) *)
-(*          | shufl t1 t2 t3 =>  shufl (repNonceMsg n n' t1) (repNonceMsg n n' t2) (repNonceMsg n n' t3) *)
-(*          (** Encryptions *) *)
-(*          | ke t1 => ke (repNonceMsg n n' t1) *)
-(*          | re t1 => re (repNonceMsg n n' t1) *)
-(*          | enc t1 t2 t3 =>  enc (repNonceMsg n n' t1) (repNonceMsg n n' t2) (repNonceMsg n n' t3) *)
-(*          | dec t1 t2 =>  dec (repNonceMsg n n' t1) (repNonceMsg n n' t2) *)
-(*            (** Blind Signatures *) *)
-(*          | kb t1 => kb (repNonceMsg n n' t1) *)
-(*          | rb t1 => rb (repNonceMsg n n' t1) *)
-(*          | bsign t1 t2 t3 =>  bsign (repNonceMsg n n' t1) (repNonceMsg n n' t2) (repNonceMsg n n' t3) *)
-(*          | bl t1 t2 t3 =>  bl (repNonceMsg n n' t1) (repNonceMsg n n' t2) (repNonceMsg n n' t3) *)
-(*          | ub t1 t2 t3 t4 => ub (repNonceMsg n n' t1) (repNonceMsg n n' t2)  (repNonceMsg n n' t3)   (repNonceMsg n n' t4) *)
-(*          (** Signatures *) *)
-(*          | ks t1 => ks (repNonceMsg n n' t1) *)
-(*          | rs t1 => rs (repNonceMsg n n' t1) *)
-(*          | sign t1 t2 t3 => sign (repNonceMsg n n' t1) (repNonceMsg n n' t2) (repNonceMsg n n' t3) *)
-(*          (* | z t1 => z t1 *) *)
-(*          | compl t1 => compl (repNonceMsg n n' t1) *)
-(*          (** all other constrs *) *)
-(*          | _ => t *)
-(*        end. *)
-
-(*   Fixpoint repNonceOs n n' os: oursum := *)
-(*     match os with *)
-(*     | msg t => msg (repNonceMsg n n' t) *)
-(*     | bol b => bol (repNonceBol n n' b) *)
-(*     end. *)
-
-(*   Fixpoint repNonceMylist n n' {m} (l: mylist m): mylist m := *)
-(*     match l with *)
-(*     | [] => [] *)
-(*     | h:t => (repNonceOs n n' h) : (repNonceMylist n n' t) *)
-(*     end. *)
-(* End aux. *)
-
-(* Section lemma_25. *)
-
-(*   Definition V (b:bool) := *)
-(*     match b with *)
-(*     | false => (V0 (nonce 0)) *)
-(*     | true => (V1 (nonce 0)) *)
-(*     end. *)
-
-(*   Definition cn (b:bool) :nat := *)
-(*     match b with *)
-(*     | false => 0 *)
-(*     | true => 1 *)
-(*     end. *)
-
-
-                      (*   Open Scope msg_scope. *)
-
-  (** **)
-(* Axiom isinCong: forall m1 m2 m3 m4, m1 # m2 -> m3 # m4 -> (isin m1 m3) ## (isin m2 m4). *)
-(* Add Parametric Morphism: (@isin) with *)
-(*     signature EQm ==> EQm ==> EQb as isin_mor. *)
-(* Proof. intros. apply isinCong; try intuition. Qed. *)
-
-(* The following frame is useful when we apply CCA2 axiom *)
-Definition z0 := phi0 ++ [msg lbl, msg (kc (nonce 3)), msg (kc (nonce 4)), msg (r 1), msg (r 2), msg pk (* public key AD*),
-                 msg (sr 14), msg (sr 15), msg (nonce 20), msg (nonce 21), msg (er 7), msg (er 8), msg (er 9), msg (er 10)].
-Arguments z0: simpl never.
-
-(* Check if a an elment of type mylist m is a sublist of mylist n without actually converting to oslist *)
-Fixpoint checkSublist {m} (l1: mylist m){n}(l2: mylist n): bool :=
-  if (m <=? n)%nat then
-    match l1 with
-    | [] => true
-    | h:t => if (checkostmylis h l2) then (checkSublist t l2) else false
-    end
-  else false.
-
-(* Occurrence indices vector *)
-Fixpoint subListPosVec {m} (l1: mylist m) {n} (l2: mylist n): Nlist:=
-  match (checkSublist l1 l2), l1 with
-  | true, h:t => (eltPos h l2)::(subListPosVec t l2)
-  | _, _ => [ ]
-  end.
-
-Axiom funcAppAttComp: forall {n} (l1 l2: mylist n) {m}(lm1 lm2: mylist m), l1 ~ l2 ->
-                                                                           ((checkSublist lm1 l1) && (checkSublist lm2 l2) = true)%bool ->
-                                                                           (subListPosVec lm1 l1) = (subListPosVec lm2 l2) ->
-                                                                           (l1 ++ [msg (f (toListm lm1))]) ~ (l2 ++ [msg (f (toListm lm2))]).
-
-Ltac tacFuncAppAttComp ml1 ml2 H:= apply funcAppAttComp with (lm1:= ml1) (lm2:= ml2) in H. 
-
-(** Given index vector retrieve sulist that constitutes elements of the positions *)
-Fixpoint getSublist (l: Nlist) {n} (ml: mylist n): mylist (length l):=
-  match l with
-  | [ ] => []
-  | h::t => (getelt_at_pos h ml): getSublist t ml
-  end.
-Axiom funcAppAttComp': forall pl {n} (l1 l2: mylist n), l1 ~ l2 -> ([msg (f (toListm (getSublist pl l1)))]++l1) ~ ([msg (f (toListm (getSublist pl l2)))] ++ l2).
-
-(* Build frame phi03 *)
-Ltac tacFuncAppAttComp' l H := apply funcAppAttComp' with (pl:= l) in H; simpl in H.
-
-(* Check hypothesis type which will be useful in computing an elt position in mylist manually *)
-Ltac chkType H :=
-  match goal with
-  | [H:?X ~ ?Y |- _ ] => let t:= type of X in idtac t "~" t
-  end.
-
-Axiom funcAppFmb: forall (p:nat) {n} (ml1 ml2 : mylist n) {f},
-    (ml1 ~ ml2) -> ([bol (f (ostomsg (getelt_at_pos p ml1)))] ++ ml1) ~ ([bol (f (ostomsg (getelt_at_pos p ml2)))] ++ ml2).
-Ltac tacFuncAppFmb g n H := apply funcAppFmb with (f:= g) (p:= n) in H; simpl in H.
-
-(* Useful to add same nonce, Vars on both sides *)
-Axiom funAppNatMsg: forall (m: nat) f {n} (ml1 ml2: mylist n), ml1 ~ ml2 -> ([msg (f m)] ++ ml1) ~ ([msg (f m)] ++ ml2).
-Ltac tacFunAppNatMsg g n H:= apply funAppNatMsg with (f:= g) (m:=n) in H; simpl in H.
 
 (** Simplified CCA2 axiom **)
-Axiom ENCCCA2': forall (n1 n2 n3: nat) (u u': message) {m} (l: mylist m),
-    (|u|#?|u'|) ## TRue ->
-    (* (List.length (distMvars l) <=? 1) = true -> *)
-    (closMylist ([msg u, msg u'] ++ l) = true) ->
-    (* cca2compmylis n n1 u u' l = true -> *)
-    (l++[msg {u}_n1^^n2]) ~ (l++ [msg {u'}_n1^^n3]).
+(* Axiom ENCCCA2': forall (n1 n2 n3: nat) (u u': message) {m} (l: mylist m), *)
+(*     (|u|#?|u'|) ## TRue -> *)
+(*     (* (List.length (distMvars l) <=? 1) = true -> *) *)
+(*     (closMylist ([msg u, msg u'] ++ l) = true) -> *)
+(*     (* cca2compmylis n n1 u u' l = true -> *) *)
+(*     (l++[msg {u}_n1^^n2]) ~ (l++ [msg {u'}_n1^^n3]). *)
 
+(* This should be provable from freshNeq *)
 Axiom bnlcheckFailForNonce: forall n t1 t2, closMsg t2 = true ->
                                             Fresh (cons n nil) [msg t2] = true -> (bnlcheck t1 (nonce n) t2) ## FAlse.
-
-(* Add morphism for bnlcheck *)
-Add Parametric Morphism :(@bnlcheck) with
-    signature EQm ==> EQm ==> EQm ==> EQb as bnlcheck_mor.
-Proof. intros; aply_cong; auto. Qed.
 
 Ltac rewBnlchkFailNonce c n1 :=
   repeat match goal with
@@ -210,6 +28,7 @@ Fixpoint and (l: list bool): bool :=
   | h::t => h || and t
   end.
 
+(* This should be provable from unforgeCommitKey *)
 Axiom isinkFalse: forall n l, let k := kc (nonce n) in
                               let l' := map (message_beq k) l in
                               and l' = false -> (isink k (f l)) ## FAlse.
@@ -218,42 +37,42 @@ Ltac tacIsinkFalse n1 :=
          | [|- context[isink (kc (nonce n1)) ?X] ] => rewrite isinkFalse with (n:= n1); try auto
          end.
 
-Ltac tacIfMorphComp:=
-  repeat match goal with
-         | [|- context[f ?X] ] => rewrite ifMorphAttComp with (l:=X); simpl; try intuition
-         end.
-
 Ltac rewAndBFalse :=
   repeat match goal with
          | [|- context [ FAlse & _ ] ] => rewrite andB_FAlse_l
          | [|- context [ _ & FAlse ] ] => rewrite andB_FAlse_r
          end; redg.
 
-Ltac tacIfMorphPair :=
-  match goal with
-  |[|- context[ (If ?B then ?T1 else ?T2, ?T3)] ] => rewrite (@ifMorphPair1 B T1 T2 T3)
-  |[|- context[ (?T1, If ?B then ?T2 else ?T3)] ] => rewrite (@ifMorphPair2 B T1 T2 T3)
-  end.
-(* Require Import Coq.Lists.List. *)
+
+Axiom ifMorphMsg: forall f b t1 t2, f (If b then t1 else t2) # (If b then (f t1) else (f t2)).
+Axiom ifMorphBol: forall f b t1 t2, f (If b then t1 else t2)  ## (IF b then (f t1) else (f t2)).
+Axiom funcAppRestr: forall p1 p2 {n m} (l1 l2: mylist m) {f: message -> message -> mylist n},
+    l1 ~ l2 ->
+    (f (ostomsg (getelt_at_pos p1 l1)) (ostomsg (getelt_at_pos p2 l1))) ~
+                                                                        (f (ostomsg (getelt_at_pos p1 l2)) (ostomsg (getelt_at_pos p2 l2))).
+Axiom funcAppRestrCompHid: forall n1 n2 v0 v1 {n} {f: message -> message -> mylist n},
+    let ml:= [msg v0, msg v1] ++ (f O O) in
+    closMylist ml = true ->
+    occur_name_mylist n1 ml = false ->
+    occur_name_mylist n2 ml = false ->
+    let c00:= (comm v0 (kc (nonce n1))) in
+    let c11:= (comm v1 (kc (nonce n2))) in
+    let c10:= (comm v1 (kc (nonce n1))) in
+    let c01:= (comm v0 (kc (nonce n2))) in
+    [msg c00, msg c11 ] ~ [msg c10, msg c01] -> (f c00 c11) ~ (f c10 c01).
+
+
 Lemma rep_first_ballot:
       let v0 := V0 (f (toListm phi0)) in
       let v1 := V1 (f (toListm phi0)) in
-      (* (| v0 |) #? (| v1 |) ## TRue -> *)
-      (vcheck v0) & (vcheck v1) ## TRue ->
-      (* let v0 := V0 (nonce 0) in *)
-      (* let v1 := V1 (nonce 0) in *)
-      (* (| v0 |) #? (| v1 |) ## TRue -> *)
-      (* Fresh [1; 2; 3; 4] [msg t, msg v0, msg v1, msg t0, msg t1] = true -> *)
-      (* closMylist [msg t] = true -> *)
-      (* (Datatypes.length (distMvars [msg t0, msg t1]) =? 2)%nat = true -> *)
-      (* bVarMylist [msg t0, msg t1] = nil -> *)
-      (* let mvl := [5; 6] in *)
-      (* mVarMsg t0 = mvl /\ mVarMsg t1 = mvl -> *)
+      (vcheck v0) & (vcheck v1) ## TRue ->  (*  which implies (| v0 |) #? (| v1 |) ## TRue -> *)
+
       (* Bothsides *)
       let r0 := (r 1) in
       let r1 := (r 2) in
       let k0 := (kc (nonce 3)) in
       let k1 := (kc (nonce 4)) in
+
       (* Left-side *)
       let c00 := (comm v0 k0) in
       let c11 := (comm v1 k1) in
@@ -272,19 +91,23 @@ Lemma rep_first_ballot:
       let e11 := (enc (pv11, TWO) (pke 11) (er 8)) in
       let phi02:= [msg b00, msg b11, msg e00, msg e11] in
       let fphi02:= f (toListm phi02) in
-      let s0 := (If (! (isin pv00 ((pi1 (d 1 fphi02)), ((pi1 (d 2 fphi02)), (pi1 (d 3 fphi02)))))) then (shufl (pi1 (d 1 fphi02)) (pi1 (d 2 fphi02)) (pi1 (d 3 fphi02))) else O)in
+      let s0 := (If (! (isin pv00 ((pi1 (d 1 fphi02)), ((pi1 (d 2 fphi02)), (pi1 (d 3 fphi02))))))
+                 then (shufl (pi1 (d 1 fphi02)) (pi1 (d 2 fphi02)) (pi1 (d 3 fphi02))) else O)in
       let dv0 := (If (dist fphi02) & (pvchecks fphi02) then s0 else |_) in
       let phi03:= phi02 ++[msg dv0] in
       let fphi03 := f (toListm phi03) in
-      let l00 := (If (bnlcheck c00 (nonce 20) fphi03) then (enc ((label c00 fphi03), (k0, THREE)) (pke 11) (er 9)) else O) in
-      let l11 := (If (bnlcheck c11 (nonce 21) fphi03) then (enc ((label c11 fphi03), (k1, THREE)) (pke 11) (er 10)) else O) in
+      let l00 := (If (bnlcheck c00 (nonce 20) fphi03)
+                  then (enc ((label c00 fphi03), (k0, THREE)) (pke 11) (er 9)) else O) in
+      let l11 := (If (bnlcheck c11 (nonce 21) fphi03)
+                  then (enc ((label c11 fphi03), (k1, THREE)) (pke 11) (er 10)) else O) in
       let phi05:= phi03++[msg l00, msg l11] in
       let fphi05 := f (toListm phi05) in
-      let do0 := (If (dist fphi05) & (pochecks fphi05) & (((isink k0 fphi05) & (isink k1 fphi05))) (* or (! ((isink k0 fphi05)or (isink k1 fphi05))))*) then (sotrm fphi05) else |_) in
+      let do0 := (If (dist fphi05) & (pochecks fphi05) & ((isink k0 fphi05) & (isink k1 fphi05)) (*or (! ((isink k0 fphi05)or (isink k1 fphi05))))*)
+                  then (sotrm fphi05) else |_) in
       let t0s0 := (If acc00 & acc11 then ((e00, (e11, dv0)), (l00, (l11, do0))) else |_) in
-  
-      (* Right-side *)  
-      let c10 := (comm v1 k0) in 
+
+      (* Right-side *)
+      let c10 := (comm v1 k0) in
       let c01 := (comm v0 k1) in
       let b10 := (bl c10 t r0) in
       let b01 := (bl c01 t r1) in
@@ -306,19 +129,15 @@ Lemma rep_first_ballot:
       let l01 := (If (bnlcheck c01 (nonce 21) fphi13) then (enc ((label c01 fphi13), (k1, THREE)) (pke 11) (er 10)) else O) in
       let phi15:= phi13++[msg l10, msg l01] in
       let fphi15 := f (toListm phi15) in
-      let do1 := (If (dist fphi15)& (pochecks fphi15)& (((isink k0 fphi15)&(isink k1 fphi15)))(* or (! ((isink k0 fphi15)or (isink k1 fphi15))))*) then (sotrm fphi15) else |_) in
+      let do1 := (If (dist fphi15)& (pochecks fphi15)& (((isink k0 fphi15)&(isink k1 fphi15))) (*or (! ((isink k0 fphi15)or (isink k1 fphi15))))*) then (sotrm fphi15) else |_) in
       let t1s1 := (If acc10 & acc01 then ((e10, (e01, dv1)), (l10, (l01, do1))) else |_) in
-      (* (occur_name_mylist 100 [msg t, msg t0, msg t1] = false) -> *)
-      (* (Fresh (cons 0 nil) [msg t, msg t2, msg t3, msg t4, msg t5] = true) -> *)
       [msg b00, msg b11, msg t0s0] ~ [msg b10, msg b01, msg t1s1].
+(*********Proof starts from here********)
+
 Proof. intros.
-       (* unfold t0s0, t1s1. unfold dv0, dv1. unfold s0, s1. *)
-       (* rewrite ifMorphIfThen.  repeat rewrite ifMorphPair2.     rewrite ifMorphPair1.  rewrite ifMorphIfThen. *)
-       (* unfold l00. *)
-       (* unfold bnlcheck. *)
-       (* unfold ncheck. *)
-            (* aply_ifbr. *) 
-    
+      
+       
+      
        aply_cca2Trans (let e00' := (enc ((c00, ((ub c00 t r0 t2), (nonce 150))), TWO) (pke 11) (er 7)) in
                        let phi02':= [msg b00, msg b11, msg e00', msg e11] in
                        let fphi02':= f (toListm phi02') in
@@ -330,7 +149,7 @@ Proof. intros.
                        let l11' := (If (bnlcheck c11 (nonce 21) fphi03') then (enc ((label c11 fphi03'), (k1, THREE)) (pke 11) (er 10)) else O) in
                        let phi05':= phi03'++[msg l00', msg l11'] in
                        let fphi05' := f (toListm phi05') in
-                       let do0' := (If (dist fphi05') & (pochecks fphi05') & (((isink k0 fphi05') & (isink k1 fphi05'))) (* or (! ((isink k0 fphi05')or (isink k1 fphi05'))))*) then (sotrm fphi05') else |_) in
+                       let do0' := (If (dist fphi05') & (pochecks fphi05') & (((isink k0 fphi05') & (isink k1 fphi05')))(* or (! ((isink k0 fphi05')or (isink k1 fphi05'))))*) then (sotrm fphi05') else |_) in
                        let t0s0' := (If acc00 & acc11 then ((e00', (e11, dv0')), (l00', (l11', do0'))) else |_) in
                        [msg b00, msg b11, msg t0s0'])
                        (let e10' := (enc ((c10, ((ub c10 t r0 t4), (nonce 150))), TWO) (pke 11) (er 7)) in
@@ -344,18 +163,40 @@ Proof. intros.
                         let l01' := (If (bnlcheck c01 (nonce 21) fphi13') then (enc ((label c01 fphi13'), (k1, THREE)) (pke 11) (er 10)) else O) in
                         let phi15':= phi13'++[msg l10', msg l01'] in
                         let fphi15' := f (toListm phi15') in
-                        let do1' := (If (dist fphi15')& (pochecks fphi15')& (((isink k0 fphi15')&(isink k1 fphi15')))(* or (! ((isink k0 fphi15')or (isink k1 fphi15'))))*) then (sotrm fphi15') else |_) in
+                        let do1' := (If (dist fphi15')& (pochecks fphi15')& (((isink k0 fphi15')&(isink k1 fphi15'))) (*or (! ((isink k0 fphi15')or (isink k1 fphi15'))))*) then (sotrm fphi15') else |_) in
                         let t1s1' := (If acc10 & acc01 then ((e10', (e01, dv1')), (l10', (l01', do1'))) else |_) in
                         [msg b10, msg b01, msg t1s1']).
 
-                      (* replace nonce in the encryption term of the left frame using CCA2, L ~ L'  *)
-       pose proof (let n1:= 11 in
-                   let n2:= 7 in
-                   let n3:= 7 in
-                   let u:= ((c00, ((ub c00 t r0 t2), (nonce 20))), TWO) in
-                   let u':= ((c00, ((ub c00 t r0 t2), (nonce 150))), TWO) in
-                   let zAdd:= [msg c00, msg c11, msg b00, msg b11,  bol (acc00&acc11), msg pv00, msg pv11, msg e11] in
-                   ENCCCA2' n1 n2 n3 u u' zAdd).
+       (* replace nonce in the encryption term of the left frame using CCA2, L ~ L'  *)
+       Axiom ENCCCA2: forall (n n1 n2 n3: nat) (u u': message) {m} (l: mylist m),
+    (|u|#?|u'|) ## TRue ->
+    (List.length (distMvars l) <=? 1) = true ->
+    distMvars l = (cons n nil) ->
+    (closMylist [msg u, msg u'] = true) ->
+    ([ n <- {u}_n1^^n2 ] l) ~ ([ n <- {u'}_n1^^n3] l).
+       pose proof (ENCCCA2 151 11 7 7 (c00, (ub c00 t r0 t2, nonce 20), TWO) (c00, (ub c00 t r0 t2, nonce 150), TWO)
+                           (let e00' := (Mvar 151) in
+                            let phi02':= [msg b00, msg b11, msg e00', msg e11] in
+                            let fphi02':= f (toListm phi02') in
+                            let s0':= (If (! (isin pv00 ((pi1 (d 1 fphi02')), ((pi1 (d 2 fphi02')), (pi1 (d 3 fphi02')))))) then (shufl (pi1 (d 1 fphi02')) (pi1 (d 2 fphi02')) (pi1 (d 3 fphi02'))) else O)in
+                            let dv0' := (If (dist fphi02') & (pvchecks fphi02') then s0' else |_) in
+                            let phi03':= phi02' ++[msg dv0'] in
+                            let fphi03' := f (toListm phi03') in
+                            let l00' := (If (bnlcheck c00 (nonce 20) fphi03') then (enc ((label c00 fphi03'), (k0, THREE)) (pke 11) (er 9)) else O) in
+                            let l11' := (If (bnlcheck c11 (nonce 21) fphi03') then (enc ((label c11 fphi03'), (k1, THREE)) (pke 11) (er 10)) else O) in
+                            let phi05':= phi03'++[msg l00', msg l11'] in
+                            let fphi05' := f (toListm phi05') in
+                            let do0' := (If (dist fphi05') & (pochecks fphi05') & (((isink k0 fphi05') & (isink k1 fphi05')))(* or (! ((isink k0 fphi05')or (isink k1 fphi05'))))*) then (sotrm fphi05') else |_) in
+                            let t0s0' := (If acc00 & acc11 then ((e00', (e11, dv0')), (l00', (l11', do0'))) else |_) in
+                            [msg b00, msg b11, msg t0s0'])) as cca2.
+
+       
+
+       simpl in cca2.
+                           If (acc00) & acc11
+        then (e00', (e11, dv0'), (l00', (l11', do0'))) 
+        else |_ in
+   [msg b00, msg b11, msg t0s0']
        simpl in H0.
        simpl in H0.
        tacFuncAppAttComp phi02 [msg b00, msg b11, msg {((c00, ((ub c00 t r0 t2), (nonce 150))), TWO)}_11^^7, msg e11] H0; try auto.
@@ -583,371 +424,175 @@ Proof. intros.
        funapp_f3bm_in ifm_then_else_ 5 2 1 H0.
        restrsublis H0; try auto.
        repeat (try apply len_reg; try rewrite eqmeql; try apply nameEql; try simpl; try intuition).
+       pose proof (let n1:= 11 in
+                   let n2:= 7 in
+                   let n3:= 7 in
+                   let u:= ((c00, ((ub c00 t r0 t2), (nonce 20))), TWO) in
+                   let u':= ((c00, ((ub c00 t r0 t2), (nonce 150))), TWO) in
+                   (*let zAdd:= [msg c00, msg c11, msg b00, msg b11,  bol (acc00&acc11), msg pv00, msg pv11, msg e11] in*)
+                   ENCCCA2' n1 n2 n3 u u' []) as cca2.
+       simpl in cca2.
+       apply funcAppRestr with (p1:=0) (p2:=1) (f:= (fun x y =>
+                                                       (let e00' := y in
+                                                        let c00 := (comm v0 k0) in
+                                                        let c11 := (comm v1 k1) in
+                                                        let phi02' := [msg b00, msg b11, msg e00', msg e11] in
+                                                        let fphi02' := f (toListm phi02') in
+                                                        let s0' :=
+                                                          If ! (isin pv00
+                                                                     (pi1 (d 1 fphi02'), (pi1 (d 2 fphi02'), pi1 (d 3 fphi02'))))
+                                                        then shufl (pi1 (d 1 fphi02')) (pi1 (d 2 fphi02'))
+                                                                   (pi1 (d 3 fphi02'))
+                                                        else O in
+                                                        let dv0' := If (dist fphi02') & (pvchecks fphi02')
+                                                        then s0'
+                                                        else |_ in
+                                                        let phi03' := phi02' ++ [msg dv0'] in
+                                                        let fphi03' := f (toListm phi03') in
+                                                        let l00' :=
+                                                              If bnlcheck c00 (nonce 20) fphi03'
+                                                        then (enc ((label c00 fphi03'), (k0, THREE)) (pke 11) (er 9))
+                                                        else O in
+                                                        let l11' :=
+                                                          If bnlcheck c11 (nonce 21) fphi03'
+                                                        then (enc ((label c11 fphi03'), (k1, THREE)) (pke 11) (er 10))
+                                                        else O in
+                                                        let phi05' := phi03' ++ [msg l00', msg l11'] in
+                                                        let fphi05' := f (toListm phi05') in
+                                                        let do0' :=     If (dist fphi05') &
+                                                                          (pochecks fphi05') & (((isink k0 fphi05')&(isink k1 fphi05'))) (* or (! ((isink k0 fphi05')or (isink k1 fphi05'))))*)
+                                                        then sotrm fphi05'
+                                                        else |_ in
+                                                        let t0s0' :=
+                                                          If (acc00) & acc11
+                                                        then (e00', (e11, dv0'), (l00', (l11', do0')))
+                                                        else |_ in
+                                                        [msg b00, msg b11, msg t0s0']))) in cca2.
+       apply cca2. repeat (try apply len_reg; try rewrite eqmeql; try apply nameEql; simpl; intuition). auto.
+
+       (* ********************* *)
+       (* replace nonce in the encryption term of the right frame using CCA2, R ~ R'  *)
+       (* ************************ *)
+       split.
+       pose proof (let n1:= 11 in
+                   let n2:= 7 in
+                   let n3:= 7 in
+                   let u:= (c10, (ub c10 t r0 t4, nonce 20), TWO) in
+                   let u':=(c10, (ub c10 t r0 t4, nonce 150), TWO) in
+                   ENCCCA2' n1 n2 n3 u u' []) as cca2.
+       simpl in cca2.
+
+apply funcAppRestr with (p1:=0) (p2:=1) (f:= (fun x y =>
+                                                           let c10 := (comm v1 k0) in
+                                                           let c01 := (comm v0 k1) in
+                                                           let e10' := y in
+                                                           let phi12' := [msg b10, msg b01, msg e10', msg e01] in
+                                                           let fphi12' := f (toListm phi12') in
+                                                           let s1' :=
+                                                             If ! (isin pv10
+                                                                        (pi1 (d 1 fphi12'), (pi1 (d 2 fphi12'), pi1 (d 3 fphi12'))))
+                                                         then shufl (pi1 (d 1 fphi12')) (pi1 (d 2 fphi12'))
+                                                                    (pi1 (d 3 fphi12'))
+                                                         else O in
+                                                         let dv1' := If (dist fphi12') & (pvchecks fphi12')
+                                                         then s1'
+                                                         else |_ in
+                                                         let phi13' := phi12' ++ [msg dv1'] in
+                                                         let fphi13' := f (toListm phi13') in
+                                                         let l10' :=
+                                                           If bnlcheck c10 (nonce 20) fphi13'
+                                                         then (enc ((label c10 fphi13'), (k0, THREE)) (pke 11) (er 9))
+                                                         else O in
+                                                         let l01' :=
+                                                           If bnlcheck c01 (nonce 21) fphi13'
+                                                         then (enc ((label c01 fphi13'), (k1, THREE)) (pke 11) (er 10))
+                                                         else O in
+                                                         let phi15' := phi13' ++ [msg l10', msg l01'] in
+                                                         let fphi15' := f (toListm phi15') in
+                                                         let do1' :=
+                                                           If (dist fphi15') &
+                                                             (pochecks fphi15') & (((isink k0 fphi15')&(isink k1 fphi15'))) (*or (! ((isink k0 fphi15')or (isink k1 fphi15')))) *)
+                                                         then sotrm fphi15'
+                                                         else |_ in
+                                                         let t1s1' :=
+                                                           If (acc10) & acc01
+                                                         then (e10', (e01, dv1'), (l10', (l01', do1')))
+                                                         else |_ in
+                                                         [msg b10, msg b01, msg t1s1'])) in cca2.
+       simpl in cca2.
+       apply cca2.  repeat (try apply len_reg; try rewrite eqmeql; try apply nameEql; simpl; intuition). auto.
        (* ********************************** *)
        (*   *********************************************************** *)
        (*   Done replacing nonce 20 using CCA2  *)
        (* Only need to prove the leftover goal *)
-       Set Nested Proofs Allowed.
-       Add Parametric Morphism :(@label) with
-           signature EQm ==> EQm ==> EQm as label_mor.
-       Proof. intros; aply_cong; auto. Qed.
-       (* This can be proved using unforgeCommitKey *) 
+       (* This can be proved using unforgeCommitKey *)
        (* Prove nonce 20 isn't there in the attacker's computation *)
        simpl.
-    
-       assert(let e00' := (enc ((c00, ((ub c00 t r0 t2), (nonce 150))), TWO) (pke 11) (er 7)) in
-              let phi02':= [msg b00, msg b11, msg e00', msg e11] in
-              let fphi02':= f (toListm phi02') in
-              let s0':= (If (! (isin pv00 ((pi1 (d 1 fphi02')), ((pi1 (d 2 fphi02')), (pi1 (d 3 fphi02'))))))
-                         then (shufl (pi1 (d 1 fphi02')) (pi1 (d 2 fphi02')) (pi1 (d 3 fphi02'))) else O)in
-              let dv0' := (If (dist fphi02') & (pvchecks fphi02') then s0' else |_) in
-              let phi03':= phi02' ++[msg dv0'] in
-              let fphi03' := f (toListm phi03') in
-              fphi03' # (If (dist fphi02') & (pvchecks fphi02')
-                         then (If (! (isin pv00 ((pi1 (d 1 fphi02')), ((pi1 (d 2 fphi02')), (pi1 (d 3 fphi02'))))))
-                               then (f (toListm (phi02'++[msg (shufl (pi1 (d 1 fphi02')) (pi1 (d 2 fphi02')) (pi1 (d 3 fphi02')))])))
-                               else (f (toListm (phi02'++[msg O]))))
-                         else (f (toListm (phi02'++[msg |_]))))).
-       simpl.
-       tacIfMorphComp.    
-       simpl in H0. repeat rewrite H0. clear H0.
-       Axiom ifMorphf2m: forall b t1 t2 t3 {f: message -> message -> message}, (f t1 (If b then t2 else t3)) # (If b then (f t1 t2) else (f t1 t3)).
-       repeat rewrite ifMorphf3.
-       repeat rewrite ifMorphf2m with (f:= label).
+
+       repeat rewrite ifMorphMsg with (f := (fun x => let e00' := (enc ((c00, ((ub c00 t r0 t2), (nonce 150))), TWO) (pke 11) (er 7)) in (f [b00; b11;e00'; e11; x]))); intuition.
+      repeat rewrite ifMorphBol.
+       repeat match goal with
+         | [|- context [label ?Y (If ?B then ?T1 else ?T2)] ] => rewrite ifMorphMsg with (f:= fun x => (label Y x))
+        end.
        rewBnlchkFailNonce c00 20.
        repeat redg.
        unfold k0.
-       tacIsinkFalse 3.  
-       rewAndBFalse. simpl.
+       tacIsinkFalse 3.
+       rewAndBFalse.
        (*************Do the same steps on right side ********)
-       (* ******************************************************** *) 
-       assert(let e10' := (enc ((c10, ((ub c10 t r0 t4), (nonce 150))), TWO) (pke 11) (er 7)) in
-              let phi12':= [msg b10, msg b01, msg e10', msg e01] in
-              let fphi12':= f (toListm phi12') in
-              let s1' := (If (! (isin pv10 ((pi1 (d 1 fphi12')), ((pi1 (d 2 fphi12')), (pi1 (d 3 fphi12'))))))
-                          then (shufl (pi1 (d 1 fphi12')) (pi1 (d 2 fphi12')) (pi1 (d 3 fphi12'))) else O) in
-              let dv1' := (If (dist fphi12') & (pvchecks fphi12') then s1' else |_) in
-              let phi13':= phi12' ++[msg dv1'] in
-              let fphi13' := f (toListm phi13') in
-              fphi13' # (If (dist fphi12') & (pvchecks fphi12') then
-                           (If (! (isin pv10 ((pi1 (d 1 fphi12')), ((pi1 (d 2 fphi12')), (pi1 (d 3 fphi12'))))))
-                            then (f (toListm (phi12'++[msg (shufl (pi1 (d 1 fphi12')) (pi1 (d 2 fphi12')) (pi1 (d 3 fphi12')))])))
-                            else (f (toListm (phi12'++[msg O])))) else (f (toListm (phi12'++[msg |_]))))).
-       simpl.
-       tacIfMorphComp.
-       simpl in H0. repeat rewrite H0.
-       repeat rewrite ifMorphf3. 
-       repeat rewrite ifMorphf2m with (f:= label).
-       rewBnlchkFailNonce c10 20. 
+       (* ******************************************************** *)
+
+       repeat rewrite ifMorphMsg with (f := (fun x => let e10' := (enc ((c10, ((ub c10 t r0 t4), (nonce 150))), TWO) (pke 11) (er 7)) in (f [b10; b01;e10'; e01; x]))); intuition.
+      repeat rewrite ifMorphBol.
+       repeat match goal with
+         | [|- context [label ?Y (If ?B then ?T1 else ?T2)] ] => rewrite ifMorphMsg with (f:= fun x => (label Y x))
+        end.
+       rewBnlchkFailNonce c10 20.
        repeat redg.
        unfold k0.
-       tacIsinkFalse 3. 
-       rewAndBFalse. simpl.  clear H0.
-                      (* repeatedly apply ifbr *)
-                      all: let n:= numgoals in idtac n.
-        repeat aply_ifbr.
-       repeat tacIfMorphPair. repeat aply_ifbr. repeat tacIfMorphComp. simpl. 
-       Axiom ifMorphf3b_fst: forall b (t1 t2 t3 t4: message) g, (g (If b then t1 else t2) t3 t4) # (If b then (g t1 t3 t4) else (g t2 t3 t4)).
-       repeat rewrite ifMorphf3b_fst with (g:= enc). repeat tacIfMorphPair. simpl.
-       repeat aply_ifbr.
-       (* Apply funcapp on comphiding *)
-       Axiom funcAppCompHid: forall {n m} (l1 l2: mylist m) {f: message -> message -> mylist n},
-           l1 ~ l2 -> (f (ostomsg (getelt_at_pos 1 l1)) (ostomsg (getelt_at_pos 2 l1))) ~ (f (ostomsg (getelt_at_pos 1 l2)) (ostomsg (getelt_at_pos 2 l2))).
-                      pose proof(compHid 3 4 v0 v1 []) as ch. simpl in ch.
-                      apply funcAppCompHid with (f:= fun x y => let b00 := (bl x t r0) in
-                                                    let b11 := (bl y t r1) in
-                                                    let t0 := (((vk 0), (Mvar 5), sign (Mvar 5) (ssk 0) (sr 14)), ((vk 1), (Mvar 6), sign (Mvar 6) (ssk 1) (sr 15))) in
-                                                    let t1 := (t0, f (cons t0 nil)) in
-                                                    let t2 := ({{ 5 := b00 }} ({{ 6:= b11 }} t0)) in
-                                                    let t3 := ({{ 5 := b00 }} ({{ 6:= b11 }} t1)) in
-                                                    let acc00 := (acc x t r0 t2) in
-                                                    let acc11 := (acc y t r1 t3) in
-                                                    let e00' := (enc ((x, ((ub x t r0 t2), (nonce 150))), TWO) (pke 11) (er 7)) in
-                                                    let e11 := (enc ((y, ((ub y t r1 t3), (nonce 21))), TWO) (pke 11) (er 8)) in
-                                                    let pv00 := (x, ((ub x t r0 t2), (nonce 20))) in
-                                                    let pv11 := (y, ((ub y t r1 t3), (nonce 21))) in
-                                                    let phi02':= [msg b00, msg b11, msg e00', msg e11] in
-                                                    let fphi02':= f (toListm phi02') in
-                                                    [msg b00, msg b11, bol (acc00) & acc11,
-                                                      bol (dist (f [b00; b11; e00'; e11])) & (pvchecks (f [b00; b11; e00'; e11])),
-                                                      bol (! (isin pv00 ((pi1 (d 1 fphi02')), ((pi1 (d 2 fphi02')), (pi1 (d 3 fphi02')))))),
-                                                      bol (IF ((dist fphi02')& (pvchecks fphi02')) then
+       tacIsinkFalse 3.
+       rewAndBFalse.
+
+
+       Ltac rewOrBFalse :=
+         repeat match goal with
+                | [|- context [ FAlse or _ ] ] => rewrite orB_FAlse_l
+                | [|- context [ _ or FAlse ] ] => rewrite orB_FAlse_r
+                end; redg.
+       rewOrBFalse.
+       pose proof(compHid 3 4 v0 v1 []) as ch. simpl in ch. simpl.
+       apply funcAppRestrCompHid with (n1:= 3) (n2:=4) (v0:= v0) (v1:= v1) (f:= fun x y => let b00 := (bl x t r0) in
+                                                 let b11 := (bl y t r1) in
+                                                 let t0 := (((vk 0), (Mvar 5), sign (Mvar 5) (ssk 0) (sr 14)), ((vk 1), (Mvar 6), sign (Mvar 6) (ssk 1) (sr 15))) in
+                                                 let t1 := (t0, f (cons t0 nil)) in
+                                                 let t2 := ({{ 5 := b00 }} ({{ 6:= b11 }} t0)) in
+                                                 let t3 := ({{ 5 := b00 }} ({{ 6:= b11 }} t1)) in
+                                                 let acc00 := (acc x t r0 t2) in
+                                                 let acc11 := (acc y t r1 t3) in
+                                                 let e00' := (enc ((x, ((ub x t r0 t2), (nonce 150))), TWO) (pke 11) (er 7)) in
+                                                 let e11 := (enc ((y, ((ub y t r1 t3), (nonce 21))), TWO) (pke 11) (er 8)) in
+                                                 let pv00 := (x, ((ub x t r0 t2), (nonce 20))) in
+                                                 let pv11 := (y, ((ub y t r1 t3), (nonce 21))) in
+                                                 let phi02':= [msg b00, msg b11, msg e00', msg e11] in
+                                                 let fphi02':= f (toListm phi02') in
+                                                 [msg b00, msg b11, msg (If (acc00) & acc11
+                                                                         then (e00', (e11,
+                                                                                       If (dist (f [b00; b11; e00'; e11])) & (pvchecks (f [b00; b11; e00'; e11]))
+                                                                                      then
+                                                                                        (If (! (isin pv00 ((pi1 (d 1 fphi02')), ((pi1 (d 2 fphi02')), (pi1 (d 3 fphi02'))))))
+                                                                                         then (shufl (pi1 (d 1 fphi02')) (pi1 (d 2 fphi02')) (pi1 (d 3 fphi02'))) else O) else |_), (O,
+                                                  (If (IF ((dist fphi02')& (pvchecks fphi02')) then
                                                              (IF (! (isin pv00 ((pi1 (d 1 fphi02')), ((pi1 (d 2 fphi02')), (pi1 (d 3 fphi02'))))))
                                                               then (bnlcheck y (nonce 21) (f [b00; b11; e00'; e11; (shufl (pi1 (d 1 fphi02')) (pi1 (d 2 fphi02')) (pi1 (d 3 fphi02')))]))
-                                                              else (bnlcheck y (nonce 21) (f [b00; b11; e00'; e11; O]))) 
-                                                           else (bnlcheck y (nonce 21) (f [b00; b11; e00'; e11; |_]))),
-                                       bol (dist (f [b00; b11; e00'; e11])) &
-                                         (pvchecks (f [b00; b11; e00'; e11])),
-                                       bol (! (isin pv00 ((pi1 (d 1 (f [b00; b11; e00'; e11]))),
-                                                           (pi1 (d 2 (f [b00; b11; e00'; e11])),
-                                                               pi1 (d 3 (f [b00; b11; e00'; e11])))))),
-                                       msg
-                                         (e00',
-                                           (e11, (shufl (pi1 (d 1 fphi02')) (pi1 (d 2 fphi02')) (pi1 (d 3 fphi02')))),
-                                           (O, ((enc ((label y (f [b00; b11; e00'; e11; (shufl (pi1 (d 1 fphi02')) (pi1 (d 2 fphi02')) (pi1 (d 3 fphi02')))])), (k1, THREE)) (pke 11) (er 10)), |_)))]) in ch.
+                                                              else (bnlcheck y (nonce 21) (f [b00; b11; e00'; e11; O])))
+                                                       else (bnlcheck y (nonce 21) (f [b00; b11; e00'; e11; |_]))) then
+                                                     (enc ( If (dist (f [b00; b11; e00'; e11])) & (pvchecks (f [b00; b11; e00'; e11]))
+                                                                                      then
+                                                                                        (If (! (isin pv00 ((pi1 (d 1 fphi02')), ((pi1 (d 2 fphi02')), (pi1 (d 3 fphi02')))))) then  (label y (f [b00; b11; e00'; e11; (shufl (pi1 (d 1 fphi02')) (pi1 (d 2 fphi02')) (pi1 (d 3 fphi02')))])) else (label y (f [b00; b11; e00'; e11; O]))) else (label y (f [b00; b11; e00'; e11; |_])), (k1, THREE)) (pke 11) (er 10)) else O, |_))) else |_)]) in ch.
+ simpl in ch.
 
-simpl in ch.
- apply ch; repeat try split; try apply vchecksImplyVoteEql; try unfold Fresh; auto. repeat try split. apply vchecksImplyVoteEql.
-auto.
-                      (* goal 2 *)
+                            apply ch. repeat try split; simpl; try apply vchecksImplyVoteEql. auto.
 
- pose proof(compHid 3 4 v0 v1 []) as ch. simpl in ch.
-                      apply funcAppCompHid with (f:= fun x y => let b00 := (bl x t r0) in
-                                                    let b11 := (bl y t r1) in
-                                                    let t0 := (((vk 0), (Mvar 5), sign (Mvar 5) (ssk 0) (sr 14)), ((vk 1), (Mvar 6), sign (Mvar 6) (ssk 1) (sr 15))) in
-                                                    let t1 := (t0, f (cons t0 nil)) in
-                                                    let t2 := ({{ 5 := b00 }} ({{ 6:= b11 }} t0)) in
-                                                    let t3 := ({{ 5 := b00 }} ({{ 6:= b11 }} t1)) in
-                                                    let acc00 := (acc x t r0 t2) in
-                                                    let acc11 := (acc y t r1 t3) in
-                                                    let e00' := (enc ((x, ((ub x t r0 t2), (nonce 150))), TWO) (pke 11) (er 7)) in
-                                                    let e11 := (enc ((y, ((ub y t r1 t3), (nonce 21))), TWO) (pke 11) (er 8)) in
-                                                    let pv00 := (x, ((ub x t r0 t2), (nonce 20))) in
-                                                    let pv11 := (y, ((ub y t r1 t3), (nonce 21))) in
-                                                    let phi02':= [msg b00, msg b11, msg e00', msg e11] in
-                                                    let fphi02':= f (toListm phi02') in
-                                                    [msg b00, msg b11, bol (acc00) & acc11,
-                                                      bol (dist (f [b00; b11; e00'; e11])) & (pvchecks (f [b00; b11; e00'; e11])),
-                                                      bol (! (isin pv00 ((pi1 (d 1 fphi02')), ((pi1 (d 2 fphi02')), (pi1 (d 3 fphi02')))))),
-                                                      bol (IF ((dist fphi02')& (pvchecks fphi02')) then
-                                                             (IF (! (isin pv00 ((pi1 (d 1 fphi02')), ((pi1 (d 2 fphi02')), (pi1 (d 3 fphi02'))))))
-                                                              then (bnlcheck y (nonce 21) (f [b00; b11; e00'; e11; (shufl (pi1 (d 1 fphi02')) (pi1 (d 2 fphi02')) (pi1 (d 3 fphi02')))]))
-                                                              else (bnlcheck y (nonce 21) (f [b00; b11; e00'; e11; O]))) 
-                                                           else (bnlcheck y (nonce 21) (f [b00; b11; e00'; e11; |_]))),
-                                       bol (dist (f [b00; b11; e00'; e11])) &
-                                         (pvchecks (f [b00; b11; e00'; e11])),
-                                       bol (! (isin pv00 ((pi1 (d 1 (f [b00; b11; e00'; e11]))),
-                                                           (pi1 (d 2 (f [b00; b11; e00'; e11])),
-                                                               pi1 (d 3 (f [b00; b11; e00'; e11])))))),
-                                       msg
-                                         (e00',
-                                           (e11, (shufl (pi1 (d 1 fphi02')) (pi1 (d 2 fphi02')) (pi1 (d 3 fphi02')))),
-                                           (O, ((enc ((label y (f [b00; b11; e00'; e11; O])), (k1, THREE)) (pke 11) (er 10)), |_)))]) in ch.
-
-simpl in ch.
-apply ch. repeat split.  apply vchecksImplyVoteEql; auto.
+Qed.
 
 
-(*** goal 3*******)
-pose proof(compHid 3 4 v0 v1 []) as ch. simpl in ch.
-                      apply funcAppCompHid with (f:= fun x y => let b00 := (bl x t r0) in
-                                                    let b11 := (bl y t r1) in
-                                                    let t0 := (((vk 0), (Mvar 5), sign (Mvar 5) (ssk 0) (sr 14)), ((vk 1), (Mvar 6), sign (Mvar 6) (ssk 1) (sr 15))) in
-                                                    let t1 := (t0, f (cons t0 nil)) in
-                                                    let t2 := ({{ 5 := b00 }} ({{ 6:= b11 }} t0)) in
-                                                    let t3 := ({{ 5 := b00 }} ({{ 6:= b11 }} t1)) in
-                                                    let acc00 := (acc x t r0 t2) in
-                                                    let acc11 := (acc y t r1 t3) in
-                                                    let e00' := (enc ((x, ((ub x t r0 t2), (nonce 150))), TWO) (pke 11) (er 7)) in
-                                                    let e11 := (enc ((y, ((ub y t r1 t3), (nonce 21))), TWO) (pke 11) (er 8)) in
-                                                    let pv00 := (x, ((ub x t r0 t2), (nonce 20))) in
-                                                    let pv11 := (y, ((ub y t r1 t3), (nonce 21))) in
-                                                    let phi02':= [msg b00, msg b11, msg e00', msg e11] in
-                                                    let fphi02':= f (toListm phi02') in
-                                                    [msg b00, msg b11, bol (acc00) & acc11,
-                                                      bol (dist (f [b00; b11; e00'; e11])) & (pvchecks (f [b00; b11; e00'; e11])),
-                                                      bol (! (isin pv00 ((pi1 (d 1 fphi02')), ((pi1 (d 2 fphi02')), (pi1 (d 3 fphi02')))))),
-                                                      bol (IF ((dist fphi02')& (pvchecks fphi02')) then
-                                                             (IF (! (isin pv00 ((pi1 (d 1 fphi02')), ((pi1 (d 2 fphi02')), (pi1 (d 3 fphi02'))))))
-                                                              then (bnlcheck y (nonce 21) (f [b00; b11; e00'; e11; (shufl (pi1 (d 1 fphi02')) (pi1 (d 2 fphi02')) (pi1 (d 3 fphi02')))]))
-                                                              else (bnlcheck y (nonce 21) (f [b00; b11; e00'; e11; O]))) 
-                                                           else (bnlcheck y (nonce 21) (f [b00; b11; e00'; e11; |_]))),
-                                       bol (dist (f [b00; b11; e00'; e11])) &
-                                         (pvchecks (f [b00; b11; e00'; e11])),
-                                                      msg
-                                         (e00',
-                                           (e11, (shufl (pi1 (d 1 fphi02')) (pi1 (d 2 fphi02')) (pi1 (d 3 fphi02')))),
-                                           (O, ((enc ((label y (f [b00; b11; e00'; e11; |_])), (k1, THREE)) (pke 11) (er 10)), |_)))]) in ch.
-
-simpl in ch.
-                      apply ch. repeat split.  apply vchecksImplyVoteEql; auto.
-                      (**********goal4*******)
-                      
-                                                               
-pose proof(compHid 3 4 v0 v1 []) as ch. simpl in ch.
-                      apply funcAppCompHid with (f:= fun x y => let b00 := (bl x t r0) in
-                                                    let b11 := (bl y t r1) in
-                                                    let t0 := (((vk 0), (Mvar 5), sign (Mvar 5) (ssk 0) (sr 14)), ((vk 1), (Mvar 6), sign (Mvar 6) (ssk 1) (sr 15))) in
-                                                    let t1 := (t0, f (cons t0 nil)) in
-                                                    let t2 := ({{ 5 := b00 }} ({{ 6:= b11 }} t0)) in
-                                                    let t3 := ({{ 5 := b00 }} ({{ 6:= b11 }} t1)) in
-                                                    let acc00 := (acc x t r0 t2) in
-                                                    let acc11 := (acc y t r1 t3) in
-                                                    let e00' := (enc ((x, ((ub x t r0 t2), (nonce 150))), TWO) (pke 11) (er 7)) in
-                                                    let e11 := (enc ((y, ((ub y t r1 t3), (nonce 21))), TWO) (pke 11) (er 8)) in
-                                                    let pv00 := (x, ((ub x t r0 t2), (nonce 20))) in
-                                                    let pv11 := (y, ((ub y t r1 t3), (nonce 21))) in
-                                                    let phi02':= [msg b00, msg b11, msg e00', msg e11] in
-                                                    let fphi02':= f (toListm phi02') in
-                                  [msg b00, msg b11, bol (acc00) & acc11,
-                                    bol (dist (f [b00; b11; e00'; e11])) & (pvchecks (f [b00; b11; e00'; e11])),
-                                    bol (! (isin pv00 ((pi1 (d 1 fphi02')), ((pi1 (d 2 fphi02')), (pi1 (d 3 fphi02')))))),
-                                    bol (IF ((dist fphi02')& (pvchecks fphi02')) then
-                                           (IF (! (isin pv00 ((pi1 (d 1 fphi02')), ((pi1 (d 2 fphi02')), (pi1 (d 3 fphi02'))))))
-                                            then (bnlcheck y (nonce 21) (f [b00; b11; e00'; e11; (shufl (pi1 (d 1 fphi02')) (pi1 (d 2 fphi02')) (pi1 (d 3 fphi02')))]))
-                                                              else (bnlcheck y (nonce 21) (f [b00; b11; e00'; e11; O]))) 
-                                                           else (bnlcheck y (nonce 21) (f [b00; b11; e00'; e11; |_]))),
-                                     
-                                                      msg
-                                         (e00',
-                                           (e11, (shufl (pi1 (d 1 fphi02')) (pi1 (d 2 fphi02')) (pi1 (d 3 fphi02')))),
-                                           (O, (O, |_)))]) in ch.
-
-simpl in ch.
-                      apply ch. repeat split.  apply vchecksImplyVoteEql; auto.
-simpl. 
-                      (*************goal 5**)
-                      
-
-pose proof(compHid 3 4 v0 v1 []) as ch. simpl in ch.
-                      apply funcAppCompHid with (f:= fun x y => let b00 := (bl x t r0) in
-                                                    let b11 := (bl y t r1) in
-                                                    let t0 := (((vk 0), (Mvar 5), sign (Mvar 5) (ssk 0) (sr 14)), ((vk 1), (Mvar 6), sign (Mvar 6) (ssk 1) (sr 15))) in
-                                                    let t1 := (t0, f (cons t0 nil)) in
-                                                    let t2 := ({{ 5 := b00 }} ({{ 6:= b11 }} t0)) in
-                                                    let t3 := ({{ 5 := b00 }} ({{ 6:= b11 }} t1)) in
-                                                    let acc00 := (acc x t r0 t2) in
-                                                    let acc11 := (acc y t r1 t3) in
-                                                    let e00' := (enc ((x, ((ub x t r0 t2), (nonce 150))), TWO) (pke 11) (er 7)) in
-                                                    let e11 := (enc ((y, ((ub y t r1 t3), (nonce 21))), TWO) (pke 11) (er 8)) in
-                                                    let pv00 := (x, ((ub x t r0 t2), (nonce 20))) in
-                                                    let pv11 := (y, ((ub y t r1 t3), (nonce 21))) in
-                                                    let phi02':= [msg b00, msg b11, msg e00', msg e11] in
-                                                    let fphi02':= f (toListm phi02') in
-                                  [msg b00, msg b11, bol (acc00) & acc11,
-                                    bol (dist (f [b00; b11; e00'; e11])) & (pvchecks (f [b00; b11; e00'; e11])),
-                                    bol (! (isin pv00 ((pi1 (d 1 fphi02')), ((pi1 (d 2 fphi02')), (pi1 (d 3 fphi02')))))),
-                                    bol (IF ((dist fphi02')& (pvchecks fphi02')) then
-                                           (IF (! (isin pv00 ((pi1 (d 1 fphi02')), ((pi1 (d 2 fphi02')), (pi1 (d 3 fphi02'))))))
-                                            then (bnlcheck y (nonce 21) (f [b00; b11; e00'; e11; (shufl (pi1 (d 1 fphi02')) (pi1 (d 2 fphi02')) (pi1 (d 3 fphi02')))]))
-                                                              else (bnlcheck y (nonce 21) (f [b00; b11; e00'; e11; O]))) 
-                                                           else (bnlcheck y (nonce 21) (f [b00; b11; e00'; e11; |_]))),
-                                     
-                                                      msg
-                                         (e00',
-                                           (e11, O),
-                                           (O, ((enc (If ((dist fphi02')& (pvchecks fphi02'))
-                                                      then (If (! (isin pv00 ((pi1 (d 1 fphi02')), ((pi1 (d 2 fphi02')), (pi1 (d 3 fphi02'))))))
-                                                            then ((label y (f [b00; b11; e00'; e11; (shufl (pi1 (d 1 fphi02')) (pi1 (d 2 fphi02')) (pi1 (d 3 fphi02')))])), (k1, THREE))
-                                                            else ((label y (f [b00; b11; e00'; e11; O])), (k1, THREE)))
-                                                      else ((label y (f [b00; b11; e00'; e11; |_])), (k1, THREE))) (pke 11) (er 10)), |_)))]) in ch.
-
-simpl in ch.
-apply ch. repeat split.  apply vchecksImplyVoteEql; auto.
-                      (** goal 6**)
-                  pose proof(compHid 3 4 v0 v1 []) as ch. simpl in ch.
-                      apply funcAppCompHid with (f:= fun x y => let b00 := (bl x t r0) in
-                                                    let b11 := (bl y t r1) in
-                                                    let t0 := (((vk 0), (Mvar 5), sign (Mvar 5) (ssk 0) (sr 14)), ((vk 1), (Mvar 6), sign (Mvar 6) (ssk 1) (sr 15))) in
-                                                    let t1 := (t0, f (cons t0 nil)) in
-                                                    let t2 := ({{ 5 := b00 }} ({{ 6:= b11 }} t0)) in
-                                                    let t3 := ({{ 5 := b00 }} ({{ 6:= b11 }} t1)) in
-                                                    let acc00 := (acc x t r0 t2) in
-                                                    let acc11 := (acc y t r1 t3) in
-                                                    let e00' := (enc ((x, ((ub x t r0 t2), (nonce 150))), TWO) (pke 11) (er 7)) in
-                                                    let e11 := (enc ((y, ((ub y t r1 t3), (nonce 21))), TWO) (pke 11) (er 8)) in
-                                                    let pv00 := (x, ((ub x t r0 t2), (nonce 20))) in
-                                                    let pv11 := (y, ((ub y t r1 t3), (nonce 21))) in
-                                                    let phi02':= [msg b00, msg b11, msg e00', msg e11] in
-                                                    let fphi02':= f (toListm phi02') in
-                                  [msg b00, msg b11, bol (acc00) & acc11,
-                                    bol (dist (f [b00; b11; e00'; e11])) & (pvchecks (f [b00; b11; e00'; e11])),
-                                    bol (! (isin pv00 ((pi1 (d 1 fphi02')), ((pi1 (d 2 fphi02')), (pi1 (d 3 fphi02')))))),
-                                    bol (IF ((dist fphi02')& (pvchecks fphi02')) then
-                                           (IF (! (isin pv00 ((pi1 (d 1 fphi02')), ((pi1 (d 2 fphi02')), (pi1 (d 3 fphi02'))))))
-                                            then (bnlcheck y (nonce 21) (f [b00; b11; e00'; e11; (shufl (pi1 (d 1 fphi02')) (pi1 (d 2 fphi02')) (pi1 (d 3 fphi02')))]))
-                                                              else (bnlcheck y (nonce 21) (f [b00; b11; e00'; e11; O]))) 
-                                                           else (bnlcheck y (nonce 21) (f [b00; b11; e00'; e11; |_]))),
-                                     
-                                                      msg
-                                         (e00',
-                                           (e11, O),
-                                           (O, (O, |_)))]) in ch.
-
-simpl in ch.
-                      apply ch. repeat split.  apply vchecksImplyVoteEql; auto.
-
-                      (** goal 7**)
-                    pose proof(compHid 3 4 v0 v1 []) as ch. simpl in ch.
-                      apply funcAppCompHid with (f:= fun x y => let b00 := (bl x t r0) in
-                                                    let b11 := (bl y t r1) in
-                                                    let t0 := (((vk 0), (Mvar 5), sign (Mvar 5) (ssk 0) (sr 14)), ((vk 1), (Mvar 6), sign (Mvar 6) (ssk 1) (sr 15))) in
-                                                    let t1 := (t0, f (cons t0 nil)) in
-                                                    let t2 := ({{ 5 := b00 }} ({{ 6:= b11 }} t0)) in
-                                                    let t3 := ({{ 5 := b00 }} ({{ 6:= b11 }} t1)) in
-                                                    let acc00 := (acc x t r0 t2) in
-                                                    let acc11 := (acc y t r1 t3) in
-                                                    let e00' := (enc ((x, ((ub x t r0 t2), (nonce 150))), TWO) (pke 11) (er 7)) in
-                                                    let e11 := (enc ((y, ((ub y t r1 t3), (nonce 21))), TWO) (pke 11) (er 8)) in
-                                                    let pv00 := (x, ((ub x t r0 t2), (nonce 20))) in
-                                                    let pv11 := (y, ((ub y t r1 t3), (nonce 21))) in
-                                                    let phi02':= [msg b00, msg b11, msg e00', msg e11] in
-                                                    let fphi02':= f (toListm phi02') in
-                                  [msg b00, msg b11, bol (acc00) & acc11,
-                                    bol (dist (f [b00; b11; e00'; e11])) & (pvchecks (f [b00; b11; e00'; e11])),
-                                    bol (IF ((dist fphi02')& (pvchecks fphi02')) then
-                                           (IF (! (isin pv00 ((pi1 (d 1 fphi02')), ((pi1 (d 2 fphi02')), (pi1 (d 3 fphi02'))))))
-                                            then (bnlcheck y (nonce 21) (f [b00; b11; e00'; e11; (shufl (pi1 (d 1 fphi02')) (pi1 (d 2 fphi02')) (pi1 (d 3 fphi02')))]))
-                                                              else (bnlcheck y (nonce 21) (f [b00; b11; e00'; e11; O]))) 
-                                                           else (bnlcheck y (nonce 21) (f [b00; b11; e00'; e11; |_]))),
-                                     
-                                                      msg
-                                         ((e00',
-                                           (e11, |_)),
-                                           (O, ((enc (If ((dist fphi02')& (pvchecks fphi02'))
-                                                      then (If (! (isin pv00 ((pi1 (d 1 fphi02')), ((pi1 (d 2 fphi02')), (pi1 (d 3 fphi02'))))))
-                                                            then ((label y (f [b00; b11; e00'; e11; (shufl (pi1 (d 1 fphi02')) (pi1 (d 2 fphi02')) (pi1 (d 3 fphi02')))])), (k1, THREE))
-                                                            else ((label y (f [b00; b11; e00'; e11; O])), (k1, THREE)))
-                                                      else ((label y (f [b00; b11; e00'; e11; |_])), (k1, THREE))) (pke 11) (er 10)), |_)))]) in ch.
-
-simpl in ch.
-                      apply ch. repeat split.  apply vchecksImplyVoteEql; auto.
-                      (** goal 8***)
-                      
-                   pose proof(compHid 3 4 v0 v1 []) as ch. simpl in ch.
-                      apply funcAppCompHid with (f:= fun x y => let b00 := (bl x t r0) in
-                                                    let b11 := (bl y t r1) in
-                                                    let t0 := (((vk 0), (Mvar 5), sign (Mvar 5) (ssk 0) (sr 14)), ((vk 1), (Mvar 6), sign (Mvar 6) (ssk 1) (sr 15))) in
-                                                    let t1 := (t0, f (cons t0 nil)) in
-                                                    let t2 := ({{ 5 := b00 }} ({{ 6:= b11 }} t0)) in
-                                                    let t3 := ({{ 5 := b00 }} ({{ 6:= b11 }} t1)) in
-                                                    let acc00 := (acc x t r0 t2) in
-                                                    let acc11 := (acc y t r1 t3) in
-                                                    let e00' := (enc ((x, ((ub x t r0 t2), (nonce 150))), TWO) (pke 11) (er 7)) in
-                                                    let e11 := (enc ((y, ((ub y t r1 t3), (nonce 21))), TWO) (pke 11) (er 8)) in
-                                                    let pv00 := (x, ((ub x t r0 t2), (nonce 20))) in
-                                                    let pv11 := (y, ((ub y t r1 t3), (nonce 21))) in
-                                                    let phi02':= [msg b00, msg b11, msg e00', msg e11] in
-                                                    let fphi02':= f (toListm phi02') in
-                                  [msg b00, msg b11, bol (acc00) & acc11,
-                                    bol (dist (f [b00; b11; e00'; e11])) & (pvchecks (f [b00; b11; e00'; e11])),
-                                    bol (IF ((dist fphi02')& (pvchecks fphi02')) then
-                                           (IF (! (isin pv00 ((pi1 (d 1 fphi02')), ((pi1 (d 2 fphi02')), (pi1 (d 3 fphi02'))))))
-                                            then (bnlcheck y (nonce 21) (f [b00; b11; e00'; e11; (shufl (pi1 (d 1 fphi02')) (pi1 (d 2 fphi02')) (pi1 (d 3 fphi02')))]))
-                                                              else (bnlcheck y (nonce 21) (f [b00; b11; e00'; e11; O]))) 
-                                                           else (bnlcheck y (nonce 21) (f [b00; b11; e00'; e11; |_]))),
-                                     
-                                                      msg
-                                         ((e00',
-                                           (e11, |_)),
-                                           (O,(O, |_)))]) in ch.
-
-simpl in ch.
-                      apply ch. repeat split.  apply vchecksImplyVoteEql; auto.
-
-                      (*** last goal ***)
-                      pose proof(compHid 3 4 v0 v1 []) as ch. simpl in ch.
-                      apply funcAppCompHid with (f:= fun x y => let b00 := (bl x t r0) in
-                                                    let b11 := (bl y t r1) in
-                                                    let t0 := (((vk 0), (Mvar 5), sign (Mvar 5) (ssk 0) (sr 14)), ((vk 1), (Mvar 6), sign (Mvar 6) (ssk 1) (sr 15))) in
-                                                    let t1 := (t0, f (cons t0 nil)) in
-                                                    let t2 := ({{ 5 := b00 }} ({{ 6:= b11 }} t0)) in
-                                                    let t3 := ({{ 5 := b00 }} ({{ 6:= b11 }} t1)) in
-                                                    let acc00 := (acc x t r0 t2) in
-                                                    let acc11 := (acc y t r1 t3) in
-     [msg b00, msg b11, bol (acc00) & acc11, msg |_]) in ch.
-apply ch. repeat split.  apply vchecksImplyVoteEql; auto.
-Qed.                                                                                          
-
-
-       
